4. (1)
   $$
   \begin{align}
   &{\begin{vmatrix}
   4&1&2&4\\
   1&2&0&2\\
   10&5&2&0\\
   0&1&1&7
   \end{vmatrix}}=
   {\begin{vmatrix}
   4&1&10&0\\
   1&2&5&1\\
   2&0&2&1\\
   4&2&0&7
   \end{vmatrix}}=
   {\begin{vmatrix}
   2&1&10&0\\
   -3&2&5&1\\
   2&0&2&1\\
   0&2&0&7
   \end{vmatrix}}\\[1em]
   
   =&{\begin{vmatrix}
   -8&1&10&0\\
   -8&2&5&1\\
   0&0&2&1\\
   0&2&0&7
   \end{vmatrix}}=
   {\begin{vmatrix}
   -8&1&10&0\\
   0&1&-5&1\\
   0&0&2&1\\
   0&2&0&7
   \end{vmatrix}}=
   {\begin{vmatrix}
   -8&1&10&0\\
   0&\frac57&-5&1\\
   0&-\frac27&2&1\\
   0&0&0&7
   \end{vmatrix}}\\[1em]
   
   =&{\begin{vmatrix}
   -8&1&10&0\\
   0&\frac57&-5&1\\
   0&0&0&\frac57\\
   0&0&0&7
   \end{vmatrix}}=0
   \end{align}
   $$
   (2)
   $$
   \begin{align}
   &{\begin{vmatrix}
   2&1&4&1\\
   3&-1&2&1\\
   1&2&3&2\\
   5&0&6&2
   \end{vmatrix}}=
   {\begin{vmatrix}
   5&1&4&1\\
   0&-1&2&1\\
   7&2&3&2\\
   5&0&6&2
   \end{vmatrix}}=
   {\begin{vmatrix}
   5&1&4&1\\
   0&-1&2&1\\
   7&2&3&2\\
   0&-1&2&1
   \end{vmatrix}}\\[1em]
   
   =&0
   \end{align}
   $$
   (3)
   $$
   \begin{align}
   &{\begin{vmatrix}
   -ab&ac&ae\\
   bd&-cd&de\\
   bf&cf&-ef
   \end{vmatrix}}=abcdef
   {\begin{vmatrix}
   -1&1&1\\
   1&-1&1\\
   1&1&-1
   \end{vmatrix}}\\[1em]
   
   =&abcdef
   {\begin{vmatrix}
   0&1&1\\
   0&-1&1\\
   2&1&-1
   \end{vmatrix}}=abcdef
   {\begin{vmatrix}
   0&1&1\\
   0&-1&1\\
   2&1&-1
   \end{vmatrix}}\\[1em]
   =&abcdef
   {\begin{vmatrix}
   2&1&1\\
   2&-1&1\\
   0&1&-1
   \end{vmatrix}}=abcdef
   {\begin{vmatrix}
   2&1&1\\
   0&-2&0\\
   0&1&-1
   \end{vmatrix}}\\[1em]
   
   =&abcdef
   {\begin{vmatrix}
   2&1&1\\
   0&-2&0\\
   0&0&-1
   \end{vmatrix}}=4abcdef
   \end{align}
   $$
   (4)
   $$
   \begin{align}
   &{\begin{vmatrix}
   1&1&1\\
   a&b&c\\
   b+c&c+a&a+b
   \end{vmatrix}}=(a+b+c)
   {\begin{vmatrix}
   1&1&1\\
   a&b&c\\
   1&1&1
   \end{vmatrix}}=0
   \end{align}
   $$
   (5)
   $$
   \begin{align}
   &{\begin{vmatrix}
   a&1&0&0\\
   -1&b&1&0\\
   0&-1&c&1\\
   0&0&-1&d
   \end{vmatrix}}=
   {\begin{vmatrix}
   a&1&0&0\\
   0&b&1&0\\
   c&-1&c&1\\
   -1&0&-1&d
   \end{vmatrix}}=
   {\begin{vmatrix}
   a&1&0&0\\
   0&b&1&0\\
   c&-1&c&1\\
   -1&0&-1&d
   \end{vmatrix}}\\[1em]
   =\frac1a&
   {\begin{vmatrix}
   a&1&0&0\\
   0&b&1&0\\
   0&-a-c&c&1\\
   -1&0&-1&d
   \end{vmatrix}}
   =\frac1{ab}
   {\begin{vmatrix}
   a&1&0&0\\
   0&b&1&0\\
   0&-a-c&c&1\\
   -1&0&-1&d
   \end{vmatrix}}\\[1em]
   =\frac1{ab}&
   {\begin{vmatrix}
   a&1&0&0\\
   0&b&1&0\\
   0&0&a+bc+c&1\\
   -1&0&-1&d
   \end{vmatrix}}=a b c d + a b + a d + c d + 1
   \end{align}
   $$
   (6)
   $$
   \begin{align}
   &{\begin{vmatrix}
   1&2&3&4\\
   1&3&4&1\\
   1&4&1&2\\
   1&1&2&3
   \end{vmatrix}}=
   {\begin{vmatrix}
   1&2&3&4\\
   0&1&1&-3\\
   1&4&1&2\\
   1&1&2&3
   \end{vmatrix}}=
   {\begin{vmatrix}
   1&2&3&4\\
   0&1&1&-3\\
   0&2&-2&-2\\
   1&1&2&3
   \end{vmatrix}}\\[1em]
   =&
   {\begin{vmatrix}
   1&2&3&4\\
   0&1&1&-3\\
   0&2&-2&-2\\
   0&-1&-1&-1
   \end{vmatrix}}=
   {\begin{vmatrix}
   1&2&3&4\\
   0&1&1&-3\\
   0&2&-2&-2\\
   0&0&0&-4
   \end{vmatrix}}=
   {\begin{vmatrix}
   1&5&3&4\\
   0&2&1&-3\\
   0&0&-2&-2\\
   0&0&0&-4
   \end{vmatrix}}\\[1em]
   =&1\times2\times(-2)\times(-4)=16
   \end{align}
   $$
   