# 习题二
## 2
$$
A=
\begin{pmatrix}
1&1&1\\
1&1&-1\\
1&-1&1
\end{pmatrix}
,\quad
B=
\begin{pmatrix}
1&2&3\\
-1&-2&4\\
0&5&1
\end{pmatrix}
$$

解：

$$
\begin{aligned}
&3AB-2A=3
{\begin{pmatrix}
1&1&1\\
1&1&-1\\
1&-1&1
\end{pmatrix}}
{\begin{pmatrix}
1&2&3\\
-1&-2&4\\
0&5&1
\end{pmatrix}}
-2
{\begin{pmatrix}
1&1&1\\
1&1&-1\\
1&-1&1
\end{pmatrix}}\\[1em]
=&
3{\begin{pmatrix}
0&5&8\\
0&-5&6\\
2&9&0
\end{pmatrix}}
-2
{\begin{pmatrix}
1&1&1\\
1&1&-1\\
1&-1&1
\end{pmatrix}}\\[1em]

=&
{\begin{pmatrix}
-2&13&22\\
-2&-17&20\\
4&29&-2
\end{pmatrix}}
\end{aligned}
$$

$$
A^TB=AB={\begin{pmatrix}
1&1&1\\
1&1&-1\\
1&-1&1
\end{pmatrix}}
{\begin{pmatrix}
1&2&3\\
-1&-2&4\\
0&5&1
\end{pmatrix}}
={\begin{pmatrix}
0&5&8\\
0&-5&6\\
2&9&0
\end{pmatrix}}
$$
## 3
$$
\begin{cases}
x_1=2y_1&&+y_3,\\
x_2=-2y_1&+3y_2&+2y_3,\\
x_3=4y_1&+y_2&+5y_3,
\end{cases}
$$
$$
\begin{cases}
y_1=-3z_1&+z_2,\\
y_2=2z_1&&+z_3,\\
y_3=&-z_2&+3z_3.
\end{cases}
$$
解：

$$
{\begin{pmatrix}
x_1\\x_2\\x_3
\end{pmatrix}}
=
{\begin{pmatrix}
2&0&1\\
-2&3&2\\
4&1&5
\end{pmatrix}}
{\begin{pmatrix}
y_1\\y_2\\y_3
\end{pmatrix}},
\quad
{\begin{pmatrix}
y_1\\y_2\\y_3
\end{pmatrix}}
=
{\begin{pmatrix}
-3&1&0\\
2&0&1\\
0&-1&3
\end{pmatrix}}
{\begin{pmatrix}
z_1\\z_2\\z_3
\end{pmatrix}}
$$

$$
\begin{aligned}
{\begin{pmatrix}
x_1\\x_2\\x_3
\end{pmatrix}}
=&
{\begin{pmatrix}
2&0&1\\
-2&3&2\\
4&1&5
\end{pmatrix}}
{\begin{pmatrix}
-3&1&0\\
2&0&1\\
0&-1&3
\end{pmatrix}}
{\begin{pmatrix}
z_1\\z_2\\z_3
\end{pmatrix}}\\[1em]

=&
{\begin{pmatrix}
-6&1&3\\
12&-4&6\\
10&-1&16
\end{pmatrix}}
{\begin{pmatrix}
z_1\\z_2\\z_3
\end{pmatrix}}
\end{aligned}
$$
## 7
$$
A=
\begin{pmatrix}
3&1\\
1&-3
\end{pmatrix}
$$
解：

$$
A^{2}
=
{\begin{pmatrix}
3&1\\
1&-3
\end{pmatrix}}
{\begin{pmatrix}
3&1\\
1&-3
\end{pmatrix}}
=
{\begin{pmatrix}
10&0\\
0&10
\end{pmatrix}}
=
10
{\begin{pmatrix}
1&0\\
0&1
\end{pmatrix}}\\[1em]

A^{50}=A^{2\times25}
=
10^{25}
{\begin{pmatrix}
1&0\\
0&1
\end{pmatrix}}\\[1em]

A^{51}=A^{50}A
=
10^{25}
{\begin{pmatrix}
3&1\\
1&-3
\end{pmatrix}}
$$
## 8
$$
(B^TAB)^T=B^TA^TB\\
\because A^T=A\\
\therefore B^TA^TB=B^TAB\\
\therefore B^TA^TB为对称矩阵
$$

若$AB$为对称矩阵，则$(AB)^T=AB$

$\Longrightarrow\ B^TA^T=AB=BA$

若$AB=BA$，则$(AB)^T=(BA)^T$

$\Longrightarrow\ AB=(AB)^T$

$\therefore\ AB=(AB)^T\Longleftrightarrow AB=BA$
## 10

$$
\begin{cases}
x_1=2y_1+2y_2+y_3,\\
x_2=3y_1+y_2+5y_3,\\
x_3=3y_1+2y_2+3y_3.
\end{cases}
$$

可得：

$$
\begin{pmatrix}
x_1\\x_2\\x_3
\end{pmatrix}
=
\begin{pmatrix}
2&2&1\\
3&1&5\\
3&2&3
\end{pmatrix}
\begin{pmatrix}
y_1\\y_2\\y_3
\end{pmatrix}
$$
$\therefore$
$$
\begin{pmatrix}
y_1\\y_2\\y_3
\end{pmatrix}
=
\begin{pmatrix}
2&2&1\\
3&1&5\\
3&2&3
\end{pmatrix}^{-1}
\begin{pmatrix}
x_1\\x_2\\x_3
\end{pmatrix}
$$
解得：
$$
\begin{pmatrix}
y_1\\y_2\\y_3
\end{pmatrix}
=
\begin{pmatrix}
2&2&1\\
3&1&5\\
3&2&3
\end{pmatrix}^{-1}
\begin{pmatrix}
x_1\\x_2\\x_3
\end{pmatrix}
$$
$\because$
$$
\begin{pmatrix}
2&2&1\\
3&1&5\\
3&2&3
\end{pmatrix}^{-1}
=
\begin{pmatrix}
-7&-4&9\\
6&3&-7\\
3&2&-4
\end{pmatrix}
$$
## 11
$$
E-J=
\begin{pmatrix}
0&-1&\cdots&-1\\
-1&0&\cdots&-1\\
\vdots&\vdots&\ddots&\vdots\\
-1&-1&\cdots&0\\
\end{pmatrix}
=
\begin{pmatrix}
1&0&\cdots&-1\\
-1&1&\cdots&-1\\
\vdots&\vdots&\ddots&\vdots\\
0&0&\cdots&0
\end{pmatrix}
=
\begin{pmatrix}
1&0&\cdots&-1\\
0&1&\cdots&-2\\
\vdots&\vdots&\ddots&\vdots\\
0&0&\cdots&-(n-1)
\end{pmatrix}=-n+1
$$
$\therefore$
$$
|E-J|=
\begin{vmatrix}
1&0&\cdots&-1\\
0&1&\cdots&-2\\
\vdots&\vdots&\ddots&\vdots\\
0&0&\cdots&-(n-1)
\end{vmatrix}=-n+1\ne0,\quad (n\ge2)
$$
$\therefore\,E-J$是可逆矩阵
$\because$
$$
(E-J)(E-\frac{1}{n-1}J)=E-(1-\frac1{n-1})J+\frac1{n-1}J^2
$$
$又\because$
$$
J^2
=
\begin{pmatrix}
1&1&\cdots&1\\
1&1&\cdots&1\\
\vdots&\vdots&\ddots&\vdots\\
1&1&\cdots&1\\
\end{pmatrix}
\begin{pmatrix}
1&1&\cdots&1\\
1&1&\cdots&1\\
\vdots&\vdots&\ddots&\vdots\\
1&1&\cdots&1\\
\end{pmatrix}
=
n
\begin{pmatrix}
1&1&\cdots&1\\
1&1&\cdots&1\\
\vdots&\vdots&\ddots&\vdots\\
1&1&\cdots&1\\
\end{pmatrix}
=
nJ
$$
$\therefore$
$$
\begin{aligned}
&(E-J)(E-\frac{1}{n-1}J)\\
=&E-(1-\frac1{n-1})J+\frac1{n-1}J^2\\
=&E-\frac n{n-1}J+\frac1{n-1}nJ\\
=&E
\end{aligned}
$$
即：$(E-J)^{-1}=E-\dfrac1{n-1}J$
## 17
$$
A
=
\begin{pmatrix}
0&3&3\\
1&1&0\\
-1&2&3
\end{pmatrix}
$$
$$
AB=A+2B
$$
$$
(A-2E)B=A
$$
$$
\begin{pmatrix}
-2&1&1\\
-1&-1&-2\\
-3&0&1
\end{pmatrix}
B
=
\begin{pmatrix}
0&3&3\\
1&1&0\\
-1&2&3
\end{pmatrix}
$$
$$
B
=
\begin{pmatrix}
0&3&3\\
1&1&0\\
-1&2&3
\end{pmatrix}
\begin{pmatrix}
-2&1&1\\
-1&-1&-2\\
-3&0&1
\end{pmatrix}^{-1}
$$
## 19
$$
A=
\begin{pmatrix}
1&0&0\\
0&-2&0\\
1&0&1
\end{pmatrix}
$$
$$
A^*BA=2BA-8E
$$
$$
|A|A^{-1}BA=2BA-8E
$$
$$
|A|A^{-1}B=2B-8A^{-1}
$$
$$
(|A|A^{-1}-2E)B=-8A^{-1}
$$
$$
B=-8A^{-1}(|A|A^{-1}-2E)^{-1}
$$
$$
B=-8(A^*-2E)A
$$
将$\begin{pmatrix}1&0&0\\0&-2&0\\1&0&1\end{pmatrix}$代入上式，解得：
$$
B=16
\begin{pmatrix}
2&0&0\\
0&-1&0\\
0&0&2
\end{pmatrix}
$$